Differentiate between reading and writing privileged registers
Allows us to check that write acess to control registers is restricted
by system access permission checks, even though they may be implicitly
read by routine operations such as address translation that don't check
system access permission.

tools/arch.ml
@@ -11,7 +11,8 @@ type isa =
     ast : Type_check.tannot def list;
     type_env : Type_check.Env.t;
     cap_regs : IdSet.t;
-    privileged_regs : IdSet.t;
+    read_privileged_regs : IdSet.t;
+    write_privileged_regs : IdSet.t;
     system_access_checks : IdSet.t;
     pcc_regs : IdSet.t;
     idc_regs : IdSet.t;
@@ -30,7 +31,8 @@ type isa =
     cap_load_funs : IdSet.t;
   }
 
-let special_regs isa = IdSet.union isa.privileged_regs (IdSet.union isa.pcc_regs isa.idc_regs)
+let privileged_regs isa = IdSet.union isa.read_privileged_regs isa.write_privileged_regs
+let special_regs isa = IdSet.union (privileged_regs isa) (IdSet.union isa.pcc_regs isa.idc_regs)
 let write_checked_regs isa = IdSet.union isa.pcc_regs isa.idc_regs
 
 let lstrip f s =
@@ -153,7 +155,8 @@ let load_isa file src_dir =
     ast;
     type_env;
     cap_regs;
-    privileged_regs = optional_idset (member "privileged_regs" arch);
+    read_privileged_regs = optional_idset (member "read_privileged_regs" arch);
+    write_privileged_regs = optional_idset (member "write_privileged_regs" arch);
     system_access_checks = optional_idset (member "system_access_checks" arch);
     pcc_regs = optional_idset (member "pcc" arch);
     idc_regs = optional_idset (member "idc" arch);
